examples/pseudo_bool/array/npbc_fullProgScript.sml
@@ -9,24 +9,6 @@ val _ = translation_extends"npbc_parseProg";
 
 val xlet_autop = xlet_auto >- (TRY( xcon) >> xsimpl)
 
-(* Translation for parsing an OPB file *)
-val r = translate tokenize_def;
-val r = translate nocomment_line_def;
-
-val nocomment_line_side_def = definition"nocomment_line_side_def";
-val nocomment_line_side = Q.prove(
-  `∀x. nocomment_line_side x <=> T`,
-  rw[nocomment_line_side_def])
-  |> update_precondition;
-
-val r = translate parse_op_def;
-val r = translate parse_constraint_def;
-val r = translate parse_constraints_def;
-
-val r = translate parse_obj_def;
-val r = translate parse_obj_maybe_def;
-val r = translate parse_pbf_toks_def;
-
 Definition noparse_string_def:
   noparse_string f s = concat[strlit"c Input file: ";f;strlit" unable to parse in format: "; s;strlit"\n"]
 End
